First generalization commit: Removed relations from lock_server.dfy

Test/591tests/lock_server.dfy
@@ -1,46 +1,57 @@
-datatype Server = Server(id:int, semaphore:bool)
-datatype Client = Client(id:int, connServers:set<int>)
-datatype DafnyState = DafnyState(clients:seq<Client>, servers:seq<Server>)
+type Id = int
 
-predicate RelationLink(m: DafnyState, c: Client, s: Server)
-{
-    && 0 <= s.id < |m.servers|
-    && 0 <= c.id < |m.clients|
-    && m.servers[s.id].id in m.clients[c.id].connServers
-}
+datatype Server = Server(id:Id, semaphore:bool)
+datatype Client = Client(id:Id, connServers:set<Server>)
+datatype DafnyState = DafnyState(clients:set<Client>, servers:set<Server>)
 
-predicate RelationSemaphore(m: DafnyState, s: Server)
-{
-    && 0 <= s.id < |m.servers|
-    && m.servers[s.id].semaphore
-}
+// predicate RelationLink(m: DafnyState, c: Client, s: Server)
+// {
+//     && 0 <= s.id < |m.servers|
+//     && 0 <= c.id < |m.clients|
+//     && m.servers[s.id].id in m.clients[c.id].connServers
 
-predicate RelationServerExists(m: DafnyState, s: Server){
-    s in m.servers
-}
+//     // forall c_: Client, s_: Server :: (c_ in m.clients && c.id == c_.id) ==> ((s_ in m.servers && s.id == s_.id) ==> s_ in c_.connServers))
+// }
 
-predicate RelationClientExists(m: DafnyState, c: Client){
-    c in m.clients
-}
+// predicate RelationSemaphore(m: DafnyState, s: Server)
+// {
+//     && 0 <= s.id < |m.servers|
+//     && m.servers[s.id].semaphore
+// }
 
-predicate RelationClientEquals(m: DafnyState, c1: Client, c2: Client){
-    && c1 in m.clients
-    && c2 in m.clients
-    && c1.id == c2.id
-}
+// predicate RelationServerExists(m: DafnyState, s: Server){
+//     s in m.servers
+// }
 
-predicate RelationServerEquals(m: DafnyState, s1: Server, s2: Server){
-    && s1 in m.servers
-    && s2 in m.servers
-    && s1.id == s2.id
-}
+// predicate RelationClientExists(m: DafnyState, c: Client){
+//     c in m.clients
+// }
+
+// predicate RelationClientEquals(m: DafnyState, c1: Client, c2: Client){
+//     && c1 in m.clients
+//     && c2 in m.clients
+//     && c1.id == c2.id
+// }
+
+// predicate RelationServerEquals(m: DafnyState, s1: Server, s2: Server){
+//     && s1 in m.servers
+//     && s2 in m.servers
+//     && s1.id == s2.id
+// }
 
 predicate Init(m: DafnyState) {
-    && (forall s: Server :: RelationServerExists(m, s) ==> RelationSemaphore(m, s))
-    && (forall s: Server, c: Client :: ((RelationServerExists(m, s) && RelationClientExists(m, c)) ==> !RelationLink(m, c, s)))
+    //&& (forall s: Server :: RelationServerExists(m, s) ==> RelationSemaphore(m, s))
+    //&& (forall s: Server, c: Client :: ((RelationServerExists(m, s) && RelationClientExists(m, c)) ==> !RelationLink(m, c, s)))
+
+    // Don't need to check IDs.
+    // Holding semaphore / connServers constant means existence of multiple items in set implies they have different IDs
+    // (because there are no duplicates)
+    && (forall s: Server :: s in m.servers ==> s.semaphore)
+    && (forall c: Client, s: Server :: (c in m.clients && s in m.servers) ==> !(s in c.connServers))
 }
 
 predicate ActionConnect(m: DafnyState, m': DafnyState) {
+    /*
 	exists c: Client, s: Server ::
         && RelationSemaphore(m, s) // in original state
         && RelationLink(m', c, s)
@@ -51,10 +62,62 @@ predicate ActionConnect(m: DafnyState, m': DafnyState) {
         
         // RelationSemaphore does not change for all other servers
         && (forall sf: Server :: (!RelationServerEquals(m, sf, s) ==> (RelationSemaphore(m, sf) == RelationSemaphore(m', sf))))
+    */
+
+    exists c: Client, c': Client, s: Server, s': Server::
+
+        && c.id == c'.id    // c and c' refer to same client
+        && s.id == s'.id    // s and s' refer to same server
+        && c in m.clients   // c is a client in the previous state
+        && c' in m'.clients // c' is a client in the next state
+        && s in m.servers   // s is a server in the previous state
+        && s' in m.servers  // s' is a server in the next state
+
+        // requirements on previous state
+        && s.semaphore // the server's semaphore is true
+
+        // requirements on next state
+        && s' in c'.connServers // the client and server are linked
+        && !s'.semaphore        // the server's semaphore is false
+
+        // requirements on the rest of the state not changing
+
+        && (forall c_: Client, c_': Client, s_: Server, s_': Server :: 
+            (
+                // c_ and s_ refer to another client server pair in the system
+                (
+                && c_ in m.clients
+                && c_' in m'.clients
+                && s_ in m.servers
+                && s_' in m'.servers
+                && c_.id == c_'.id
+                && s_.id == s_'.id
+                && (c_.id != c.id || s_.id != s.id)
+                )
+                ==>
+                // link between client and server doesn't change
+                ((s_ in c_.connServers) == (s_' in c_'.connServers))
+            )
+        )
+        
+        && (forall s_: Server, s_': Server ::
+            (
+                // s_ refers to another server in the system
+                (
+                && s_ in m.servers
+                && s_' in m'.servers
+                && s_.id == s_'.id
+                && s_.id != s.id
+                )
+                ==>
+                // server's semaphore doesn't change
+                (s_.semaphore == s_'.semaphore)
+            )
+        )
 }
 
 predicate ActionDisconnect(m: DafnyState, m': DafnyState) {
-    exists c: Client, s: Server ::
+    /*exists c: Client, s: Server ::
 		&& RelationLink(m, c, s)
         && !RelationLink(m', c, s)
         && RelationSemaphore(m', s)
@@ -64,6 +127,58 @@ predicate ActionDisconnect(m: DafnyState, m': DafnyState) {
         
         // RelationSemaphore does not change for all other servers
         && (forall sf: Server :: (!RelationServerEquals(m, sf, s) ==> (RelationSemaphore(m, sf) == RelationSemaphore(m', sf))))
+    */
+        exists c: Client, c': Client, s: Server, s': Server::
+
+            && c.id == c'.id    // c and c' refer to same client
+            && s.id == s'.id    // s and s' refer to same server
+            && c in m.clients   // c is a client in the previous state
+            && c' in m'.clients // c' is a client in the next state
+            && s in m.servers   // s is a server in the previous state
+            && s' in m.servers  // s' is a server in the next state
+
+            // requirements on previous state
+            && s in c.connServers // the client and server are linked
+
+            // requirements on next state
+            && !(s' in c'.connServers) // the client and server are not linked
+            && s'.semaphore            // the server's semaphore is true
+
+            // requirements on the rest of the state not changing
+
+            && (forall c_: Client, c_': Client, s_: Server, s_': Server :: 
+                (
+                    // c_ and s_ refer to another client server pair in the system
+                    (
+                    && c_ in m.clients
+                    && c_' in m'.clients
+                    && s_ in m.servers
+                    && s_' in m'.servers
+                    && c_.id == c_'.id
+                    && s_.id == s_'.id
+                    && (c_.id != c.id || s_.id != s.id)
+                    )
+                    ==>
+                    // link between client and server doesn't change
+                    ((s_ in c_.connServers) == (s_' in c_'.connServers))
+                )
+            )
+            
+            && (forall s_: Server, s_': Server ::
+                (
+                    // s_ refers to another server in the system
+                    (
+                    && s_ in m.servers
+                    && s_' in m'.servers
+                    && s_.id == s_'.id
+                    && s_.id != s.id
+                    )
+                    ==>
+                    // server's semaphore doesn't change
+                    (s_.semaphore == s_'.semaphore)
+                )
+            )
+        
 }
 
 predicate Next(m:DafnyState, m':DafnyState) {
@@ -74,7 +189,11 @@ predicate Next(m:DafnyState, m':DafnyState) {
 
 predicate Safety(m: DafnyState)
 {
-    forall c1: Client, c2:Client, s: Server :: ((RelationClientExists(m, c1) && RelationClientExists(m, c2) && RelationServerExists(m, s)) ==> ((RelationLink(m, c1, s) && RelationLink(m, c2, s)) ==> RelationClientEquals(m, c1, c2)))
+    // forall c1: Client, c2:Client, s: Server :: ((RelationClientExists(m, c1) && RelationClientExists(m, c2) && RelationServerExists(m, s)) ==> ((RelationLink(m, c1, s) && RelationLink(m, c2, s)) ==> RelationClientEquals(m, c1, c2)))
+    forall c1: Client, c2: Client, s: Server :: (
+        (c1 in m.clients && c2 in m.clients && s in m.servers) ==>
+        ((s in c1.connServers && s in c2.connServers) ==> c1.id == c2.id)
+    )
 }
 
 /*
